-

RingLike.v
@@ -50,7 +50,7 @@ Class ring_like_op T :=
     rngl_one : T;
     rngl_add : T → T → T;
     rngl_mul : T → T → T;
-    rngl_opt_opp' : T → option T;
+    rngl_opt_opp : T → option T;
     rngl_opt_inv : T → option T;
     rngl_opt_sous : option (T → T → T);
     rngl_opt_quot : option (T → T → T);
@@ -65,23 +65,24 @@ Definition map_option {T} d (x : option T) :=
   | None => d
   end.
 
-Arguments rngl_opt_opp' {T}%type {ring_like_op} a%F.
+Arguments rngl_opt_opp {T}%type {ring_like_op} a%F.
+Arguments rngl_opt_inv {T}%type {ring_like_op} a%F.
 
-Definition rngl_opp' {T} {R : ring_like_op T} a :=
-  map_option rngl_zero (rngl_opt_opp' a).
+Definition rngl_opp {T} {R : ring_like_op T} a :=
+  map_option rngl_zero (rngl_opt_opp a).
 Definition rngl_inv {T} {R : ring_like_op T} a :=
   map_option rngl_zero (rngl_opt_inv a).
 
-Definition rngl_opp_defined' {T} {R : ring_like_op T} a :=
-  bool_of_option (rngl_opt_opp' a).
+Definition rngl_opp_defined {T} {R : ring_like_op T} a :=
+  bool_of_option (rngl_opt_opp a).
 Definition rngl_inv_defined {T} {R : ring_like_op T} a :=
   bool_of_option (rngl_opt_inv a).
 
-Arguments rngl_opp_defined' {T}%type {R} a%F.
+Arguments rngl_opp_defined {T}%type {R} a%F.
 Arguments rngl_inv_defined {T}%type {R} a%F.
 
 Definition rngl_is_ring {T} {R : ring_like_op T} :=
-  ∀ x, rngl_opp_defined' x = true.
+  ∀ x, rngl_opp_defined x = true.
 
 Definition rngl_is_field {T} {R : ring_like_op T} :=
   ∀ x, x = rngl_zero ∨ rngl_inv_defined x = true.
@@ -104,8 +105,8 @@ Definition rngl_quot {T} {R : ring_like_op T} a b :=
   | None => rngl_zero
   end.
 
-Definition rngl_sub' {T} {R : ring_like_op T} a b :=
-  if rngl_opp_defined' b then rngl_add a (rngl_opp' b) else rngl_zero.
+Definition rngl_sub {T} {R : ring_like_op T} a b :=
+  if rngl_opp_defined b then rngl_add a (rngl_opp b) else rngl_zero.
 
 Definition rngl_div {T} {R : ring_like_op T} a b :=
   if rngl_inv_defined b then rngl_mul a (rngl_inv b) else rngl_zero.
@@ -113,17 +114,17 @@ Definition rngl_div {T} {R : ring_like_op T} a b :=
 Notation "0" := rngl_zero : ring_like_scope.
 Notation "1" := rngl_one : ring_like_scope.
 Notation "a + b" := (rngl_add a b) : ring_like_scope.
-Notation "a - b" := (rngl_sub' a b) : ring_like_scope.
+Notation "a - b" := (rngl_sub a b) : ring_like_scope.
 Notation "a * b" := (rngl_mul a b) : ring_like_scope.
 Notation "a / b" := (rngl_div a b) : ring_like_scope.
 Notation "a ≤ b" := (rngl_le a b) : ring_like_scope.
-Notation "- a" := (rngl_opp' a) : ring_like_scope.
+Notation "- a" := (rngl_opp a) : ring_like_scope.
 Notation "a '⁻¹'" := (rngl_inv a) (at level 35, right associativity, format "a ⁻¹") :
   ring_like_scope.
 Notation "a ≤ b ≤ c" := (a ≤ b ∧ b ≤ c)%F (at level 70, b at next level) :
   ring_like_scope.
 
-Notation "- 1" := (rngl_opp' rngl_one) : ring_like_scope.
+Notation "- 1" := (rngl_opp rngl_one) : ring_like_scope.
 
 Inductive not_applicable := NA.
 
@@ -160,14 +161,18 @@ Class ring_like_prop T {ro : ring_like_op T} :=
        ∀ a b c, ((a + b) * c = a * c + b * c)%F;
     (* properties of general opposite and general inverse *)
     rngl_opt_opp_iff :
-      ∀ a b, rngl_opt_opp' a = Some b ↔ (a + b = 0)%F;
+      ∀ a b, rngl_opt_opp a = Some b ↔ (a + b = 0)%F;
+    rngl_opt_inv_l_iff :
+      ∀ a b, rngl_opt_inv a = Some b ↔ (b * a = 1)%F;
+    rngl_opt_inv_r_iff :
+      if rngl_is_comm then not_applicable
+      else ∀ a b, rngl_opt_inv a = Some b ↔ (a * b = 1)%F;
 (*
     rngl_opp_defined_add :
       ∀ a b,
       rngl_opp_defined a = true
       → rngl_opp_defined b = true
       → rngl_opp_defined (a + b) = true;
-*)
     rngl_opt_inv_symm :
       ∀ a b, rngl_opt_inv a = Some b → rngl_opt_inv b = Some a;
     rngl_inv_defined_mul :
@@ -175,6 +180,7 @@ Class ring_like_prop T {ro : ring_like_op T} :=
       rngl_inv_defined a = true
       → rngl_inv_defined b = true
       → rngl_inv_defined (a * b) = true;
+*)
     (* when has opposite *)
 (*
     rngl_opt_add_opp_l :
@@ -328,23 +334,23 @@ destruct ic. {
 Qed.
 
 Theorem rngl_add_opp_l : ∀ a,
-  rngl_opp_defined' a = true →
+  rngl_opp_defined a = true →
   (- a + a = 0)%F.
 Proof.
 intros * H1.
 rewrite rngl_add_comm.
 apply rngl_opt_opp_iff.
-unfold rngl_opp_defined' in H1.
-remember (rngl_opt_opp' a) as b eqn:Hb.
+unfold rngl_opp_defined in H1.
+remember (rngl_opt_opp a) as b eqn:Hb.
 symmetry in Hb.
 destruct b as [b| ]; [ | easy ].
 clear H1.
-unfold rngl_opp'.
+unfold rngl_opp.
 now rewrite Hb.
 Qed.
 
 Theorem rngl_add_opp_r : ∀ a,
-  rngl_opp_defined' a = true →
+  rngl_opp_defined a = true →
   (a + - a = 0)%F.
 Proof.
 intros * H1.
@@ -469,23 +475,23 @@ now rewrite Hab.
 Qed.
 
 Theorem fold_rngl_sub : ∀ a b,
-  rngl_opp_defined' b = true →
+  rngl_opp_defined b = true →
   (a + - b)%F = (a - b)%F.
 Proof.
 intros * Hro.
-unfold rngl_sub'.
+unfold rngl_sub.
 now rewrite Hro.
 Qed.
 
 Theorem rngl_sub_diag : ∀ a,
-  rngl_opp_defined' a = true ∨ rngl_has_sous = true →
+  rngl_opp_defined a = true ∨ rngl_has_sous = true →
   (a - a = 0)%F.
 Proof.
 intros * Hom.
-remember (rngl_opp_defined' a) as op eqn:Hop.
+remember (rngl_opp_defined a) as op eqn:Hop.
 symmetry in Hop.
 destruct op. {
-  unfold rngl_sub'.
+  unfold rngl_sub.
   rewrite Hop.
   rewrite rngl_add_comm.
   now apply rngl_add_opp_l.
@@ -502,14 +508,14 @@ now destruct Hom.
 Qed.
 
 Theorem rngl_add_sub : ∀ a b,
-  rngl_opp_defined' b = true ∨ rngl_has_sous = true →
+  rngl_opp_defined b = true ∨ rngl_has_sous = true →
   (a + b - b = a)%F.
 Proof.
 intros * Hom.
-remember (rngl_opp_defined' b) as op eqn:Hop.
+remember (rngl_opp_defined b) as op eqn:Hop.
 symmetry in Hop.
 destruct op. {
-  unfold rngl_sub'.
+  unfold rngl_sub.
   rewrite Hop.
   rewrite <- rngl_add_assoc.
   rewrite (rngl_add_comm b).
@@ -526,16 +532,16 @@ now destruct Hom.
 Qed.
 
 Theorem rngl_add_cancel_l : ∀ a b c,
-  rngl_opp_defined' a = true ∨ rngl_has_sous = true →
+  rngl_opp_defined a = true ∨ rngl_has_sous = true →
   (a + b = a + c)%F → (b = c)%F.
 Proof.
 intros * Hom Habc.
-remember (rngl_opp_defined' a) as op eqn:Hop.
+remember (rngl_opp_defined a) as op eqn:Hop.
 symmetry in Hop.
 destruct op. {
-  apply (f_equal (λ x, rngl_sub' x a)) in Habc.
+  apply (f_equal (λ x, rngl_sub x a)) in Habc.
   do 2 rewrite (rngl_add_comm a) in Habc.
-  unfold rngl_sub' in Habc.
+  unfold rngl_sub in Habc.
   rewrite Hop in Habc.
   do 2 rewrite <- rngl_add_assoc in Habc.
   rewrite fold_rngl_sub in Habc; [ | easy ].
@@ -556,7 +562,7 @@ now destruct Hom.
 Qed.
 
 Theorem rngl_add_sub_eq_l : ∀ a b c,
-  rngl_opp_defined' a = true ∨ rngl_has_sous = true →
+  rngl_opp_defined a = true ∨ rngl_has_sous = true →
   (a + b = c → c - a = b)%F.
 Proof.
 intros * Hom Hab.
@@ -566,7 +572,7 @@ now apply rngl_add_sub.
 Qed.
 
 Theorem rngl_add_sub_eq_r : ∀ a b c,
-  rngl_opp_defined' b = true ∨ rngl_has_sous = true →
+  rngl_opp_defined b = true ∨ rngl_has_sous = true →
    (a + b = c → c - b = a)%F.
 Proof.
 intros * Hom Hab.
@@ -582,7 +588,7 @@ now rewrite Hab.
 Qed.
 
 Theorem rngl_add_cancel_r : ∀ a b c,
-  rngl_opp_defined' c = true ∨ rngl_has_sous = true →
+  rngl_opp_defined c = true ∨ rngl_has_sous = true →
   (a + c = b + c)%F → (a = b)%F.
 Proof.
 intros * Hom Habc.
@@ -591,7 +597,7 @@ now do 2 rewrite rngl_add_sub in Habc.
 Qed.
 
 Theorem rngl_mul_0_r : ∀ a,
-  rngl_opp_defined' a = true ∨ rngl_has_sous = true →
+  rngl_opp_defined a = true ∨ rngl_has_sous = true →
   (a * 0 = 0)%F.
 Proof.
 intros * Hom.
@@ -601,7 +607,7 @@ now do 2 rewrite rngl_add_0_l.
 Qed.
 
 Theorem rngl_mul_0_l : ∀ a,
-  rngl_opp_defined' a = true ∨ rngl_has_sous = true →
+  rngl_opp_defined a = true ∨ rngl_has_sous = true →
   (0 * a = 0)%F.
 Proof.
 intros * Hom.
@@ -611,14 +617,14 @@ now do 2 rewrite rngl_add_0_l.
 Qed.
 
 Theorem rngl_add_move_0_r : ∀ a b,
-  rngl_opp_defined' b = true →
+  rngl_opp_defined b = true →
   (a + b = 0)%F ↔ (a = - b)%F.
 Proof.
 intros * Hro.
 split; intros H. {
   apply rngl_sub_compat_l with (c := b) in H.
   rewrite rngl_add_sub in H; [ | now left ].
-  unfold rngl_sub' in H.
+  unfold rngl_sub in H.
   rewrite Hro in H.
   now rewrite rngl_add_0_l in H.
 } {
@@ -628,8 +634,8 @@ split; intros H. {
 Qed.
 
 Theorem rngl_opt_opp_symm : ∀ a b,
-  rngl_opt_opp' a = Some b
-  → rngl_opt_opp' b = Some a.
+  rngl_opt_opp a = Some b
+  → rngl_opt_opp b = Some a.
 Proof.
 intros * Hab.
 apply rngl_opt_opp_iff in Hab.
@@ -637,32 +643,88 @@ rewrite rngl_add_comm in Hab.
 now apply rngl_opt_opp_iff in Hab.
 Qed.
 
+Theorem rngl_opt_inv_iff : ∀ a b,
+  rngl_opt_inv a = Some b ↔ (a * b = 1)%F ∧ (b * a = 1)%F.
+Proof.
+intros.
+split; intros Hab. {
+  split. {
+    remember rngl_is_comm as ic eqn:Hic.
+    symmetry in Hic.
+    destruct ic. {
+      rewrite rngl_mul_comm; [ | easy ].
+      now apply rngl_opt_inv_l_iff in Hab.
+    } {
+      specialize rngl_opt_inv_r_iff as H1.
+      rewrite Hic in H1.
+      now apply H1.
+    }
+  } {
+    now apply rngl_opt_inv_l_iff.
+  }
+} {
+  destruct Hab as (Hab, Hba).
+  now apply rngl_opt_inv_l_iff.
+}
+Qed.
+
+Theorem rngl_opt_inv_symm : ∀ a b,
+  rngl_opt_inv a = Some b
+  → rngl_opt_inv b = Some a.
+Proof.
+intros * Hab.
+apply rngl_opt_inv_iff in Hab.
+now apply rngl_opt_inv_iff.
+Qed.
+
 Theorem rngl_opp_defined_opp : ∀ a,
-  rngl_opp_defined' a = true
-  → rngl_opp_defined' (- a) = true.
+  rngl_opp_defined a = true
+  → rngl_opp_defined (- a) = true.
 Proof.
 intros * Hro.
-unfold rngl_opp_defined' in Hro |-*.
+unfold rngl_opp_defined in Hro |-*.
 unfold bool_of_option in Hro |-*.
-remember (rngl_opt_opp' a) as oa eqn:Hoa.
+remember (rngl_opt_opp a) as oa eqn:Hoa.
 symmetry in Hoa.
 destruct oa as [a'| ]; [ | easy ].
 apply rngl_opt_opp_symm in Hoa.
-remember (rngl_opt_opp' (- a)%F) as oa eqn:Hoa'.
+remember (rngl_opt_opp (- a)) as oa eqn:Hoa'.
 symmetry in Hoa'.
 destruct oa as [a''| ]; [ easy | ].
 apply rngl_opt_opp_symm in Hoa.
-unfold rngl_opp' in Hoa'.
+unfold rngl_opp in Hoa'.
 rewrite Hoa in Hoa'.
 unfold map_option in Hoa'.
 apply rngl_opt_opp_symm in Hoa.
 now rewrite Hoa in Hoa'.
 Qed.
 
+Theorem rngl_inv_defined_inv : ∀ a,
+  rngl_inv_defined a = true
+  → rngl_inv_defined (a⁻¹) = true.
+Proof.
+intros * Hro.
+unfold rngl_inv_defined in Hro |-*.
+unfold bool_of_option in Hro |-*.
+remember (rngl_opt_inv a) as ia eqn:Hia.
+symmetry in Hia.
+destruct ia as [a'| ]; [ | easy ].
+apply rngl_opt_inv_symm in Hia.
+remember (rngl_opt_inv (a⁻¹)) as ia eqn:Hia'.
+symmetry in Hia'.
+destruct ia as [a''| ]; [ easy | ].
+apply rngl_opt_inv_symm in Hia.
+unfold rngl_inv in Hia'.
+rewrite Hia in Hia'.
+unfold map_option in Hia'.
+apply rngl_opt_inv_symm in Hia.
+now rewrite Hia in Hia'.
+Qed.
+
 Theorem rngl_opp_add_prop : ∀ a b a' b',
-  rngl_opt_opp' a = Some a' →
-  rngl_opt_opp' b = Some b' →
-  rngl_opt_opp' (a + b) = Some (b' + a')%F.
+  rngl_opt_opp a = Some a' →
+  rngl_opt_opp b = Some b' →
+  rngl_opt_opp (a + b) = Some (b' + a')%F.
 Proof.
 intros * Ha Hb.
 apply rngl_opt_opp_iff in Ha.
@@ -673,10 +735,25 @@ rewrite <- (rngl_add_assoc a).
 now rewrite Hb, rngl_add_0_r.
 Qed.
 
+Theorem rngl_inv_mul_prop : ∀ a b a' b',
+  rngl_opt_inv a = Some a' →
+  rngl_opt_inv b = Some b' →
+  rngl_opt_inv (a * b) = Some (b' * a')%F.
+Proof.
+intros * Ha Hb.
+apply rngl_opt_inv_l_iff in Ha.
+apply rngl_opt_inv_l_iff in Hb.
+apply rngl_opt_inv_l_iff.
+rewrite rngl_mul_assoc.
+rewrite <- (rngl_mul_assoc b').
+rewrite Ha.
+now rewrite rngl_mul_1_r.
+Qed.
+
 Theorem rngl_opp_mul_prop : ∀ a b a' b',
-  rngl_opt_opp' a = Some a' →
-  rngl_opt_opp' b = Some b' →
-  rngl_opt_opp' (a * b) = Some (a' * b')%F.
+  rngl_opt_opp a = Some a' →
+  rngl_opt_opp b = Some b' →
+  rngl_opt_opp (a * b) = Some (a' * b')%F.
 Proof.
 intros * Ha Hb.
 apply rngl_opt_opp_iff in Ha.
